Capybara/Syntax/CaptureSet.lean
@@ -1,1 +1,2 @@
 import Capybara.Syntax.CaptureSet.Core
+import Capybara.Syntax.CaptureSet.Subst
