Capybara/Syntax/CaptureSet/Subst.lean
@@ -1,0 +1,15 @@
+import Capybara.Syntax.CaptureSet.Core
+import Capybara.Morphism.Subst
+namespace Capybara
+
+def CaptureSet.subst
+  (C : CaptureSet n k)
+  (σ : Subst n m k n' m' k') :
+  CaptureSet n' k' :=
+  match C with
+  | empty => {}
+  | union C1 C2 => (C1.subst σ) ∪ (C2.subst σ)
+  | singleton x m => {x@m:=σ.var x}
+  | csingleton c m => (σ.cvar c).qualified m
+
+end Capybara
