Capybara/Syntax/Type/Subst.lean
@@ -1,0 +1,24 @@
+import Capybara.Morphism.Subst
+import Capybara.Syntax.Type.Core
+namespace Capybara
+
+mutual
+
+def EType.subst
+  (E : EType n m k)
+  (σ : Subst n m k n' m' k') :
+  EType n' m' k' := sorry
+
+def CType.subst
+  (T : CType n m k)
+  (σ : Subst n m k n' m' k') :
+  CType n' m' k' := sorry
+
+def SType.subst
+  (S : SType n m k)
+  (σ : Subst n m k n' m' k') :
+  SType n' m' k' := sorry
+
+end
+
+end Capybara
